examples/logic/ltl/generalHelpersScript.sml
@@ -270,10 +270,11 @@ val CAT_OPTIONS_def = Define`
 val CAT_OPTIONS_MAP_LEMM = store_thm
   ("CAT_OPTIONS_MAP_LEMM",
    ``!i f ls. MEM i (CAT_OPTIONS (MAP f ls))
-  ==> ?x. MEM x ls ∧ (SOME i = f x)``,
+  = ?x. MEM x ls ∧ (SOME i = f x)``,
    Induct_on `ls` >> fs[CAT_OPTIONS_def,MAP]
-   >> rpt strip_tac >> Cases_on `IS_SOME (f h)`
-   >> fs[IS_SOME_EXISTS] >> rw[] >> fs[CAT_OPTIONS_def] >> metis_tac[]
+   >> rpt strip_tac >> Cases_on `IS_SOME (f h)` >> simp[EQ_IMP_THM]
+   >> fs[IS_SOME_EXISTS] >> rw[] >> fs[CAT_OPTIONS_def]
+   >> metis_tac[SOME_11,NOT_SOME_NONE]
   );
 
 val OPTION_TO_LIST_def = Define`
@@ -320,7 +321,7 @@ val FIND_LEMM = store_thm
 
 val FIND_LEMM2 = store_thm
   ("FIND_LEMM2",
-   ``!P x l. (FIND P l = SOME x) ==> (MEM x l)``,
+   ``!P x l. (FIND P l = SOME x) ==> (MEM x l ∧ P x)``,
    gen_tac >> Induct_on `l` >> fs[FIND_def,INDEX_FIND_def]
    >> rpt strip_tac >> Cases_on `P h` >> fs[] >> Cases_on `z`
    >> fs[]
